src/mqtt-packet-parser/src/connect.fst
@@ -1,6 +1,7 @@
 module Connect
 
 module U8 = FStar.UInt8
+module U16 = FStar.UInt16
 module U32 = FStar.UInt32
 module B = LowStar.Buffer
 
@@ -8,9 +9,11 @@ open C.String
 open LowStar.BufferOps
 open FStar.HyperStack.ST
 open FStar.Int.Cast
+open LowStar.Printf
 
 open Const
 open Common
+open Debug_FFI
 
 
 val assemble_connect_struct: s: struct_connect_parts
@@ -27,7 +30,6 @@ let assemble_connect_struct s =
   let will_flag: U8.t = slice_byte connect_flag 5uy 6uy in
   let clean_start_flag: U8.t = slice_byte connect_flag 6uy 7uy in
   let resreved_flag: U8.t = slice_byte connect_flag 7uy 8uy in
-  let connect_property_id: U8.t = s.connect_connect_property_id in
   {
     message_type = connect_constant.message_type_constant;
     message_name = connect_constant.message_name_constant;
@@ -52,26 +54,7 @@ let assemble_connect_struct s =
             clean_start = clean_start_flag;
           };
           keep_alive = s.connect_keep_alive;
-          connect_topic_length = s.connect_connect_topic_length;
-          connect_property =
-          if (U8.eq connect_property_id define_connect_property_session_expiry_interval_id) then 
-            define_struct_connect_property_session_expiry_interval
-          else if (U8.eq connect_property_id define_connect_property_receive_maximum_id) then 
-            define_struct_connect_property_receive_maximum
-          else if (U8.eq connect_property_id define_connect_property_maximum_packet_size_id) then 
-            define_struct_connect_property_maximum_packet_size
-          else if (U8.eq connect_property_id define_connect_property_topic_alias_maximum_id) then 
-            define_struct_connect_property_topic_alias_maximum
-          else if (U8.eq connect_property_id define_connect_property_request_response_information_id) then 
-            define_struct_connect_property_request_response_information
-          else if (U8.eq connect_property_id define_connect_property_request_problem_information_id) then 
-            define_struct_connect_property_request_problem_information    
-          else if (U8.eq connect_property_id define_connect_property_user_property_id) then 
-            define_struct_connect_property_user_property
-          else if (U8.eq connect_property_id define_connect_property_authentication_method_id) then 
-            define_struct_connect_property_authentication_method
-          else
-            define_struct_connect_property_authentication_data
+          connect_id = s.connect_id;
         };
     publish = {
       topic_length = 0ul;
@@ -82,12 +65,77 @@ let assemble_connect_struct s =
       property_id = max_u8;
     };
     disconnect = define_struct_disconnect_error;
-    property = property_struct_base;
+    property = s.connect_property;
     error = {
       code = define_no_error_code;
       message = define_no_error;
     };
   }
+
+val is_valid_protocol_name: packet_data: (B.buffer U8.t) 
+  -> next_start_index:U32.t
+  -> Stack (protocoll_name_struct: struct_protocol_name)
+    (requires fun h0 -> B.live h0 packet_data)
+    (ensures fun h0 r h1 -> true)
+let is_valid_protocol_name packet_data next_start_index = 
+  (
+    if (
+        (not (U8.eq packet_data.(U32.(next_start_index +^ 0ul)) 0x00uy)) ||
+        (not (U8.eq packet_data.(U32.(next_start_index +^ 1ul)) 0x04uy)) ||
+        (not (U8.eq packet_data.(U32.(next_start_index +^ 2ul)) 0x4Duy)) ||
+        (not (U8.eq packet_data.(U32.(next_start_index +^ 3ul)) 0x51uy)) ||
+        (not (U8.eq packet_data.(U32.(next_start_index +^ 4ul)) 0x54uy)) ||
+        (not (U8.eq packet_data.(U32.(next_start_index +^ 5ul)) 0x54uy))
+      ) then
+      (
+        let protocoll_name_struct: struct_protocol_name = {
+          is_valid_protocol_name = false;
+          protocol_version_start_index = 0ul;
+        } in protocoll_name_struct
+      )
+    else 
+      (
+        let protocoll_name_struct: struct_protocol_name = {
+          is_valid_protocol_name = true;
+          protocol_version_start_index = U32.(next_start_index +^ 6ul);
+        } in protocoll_name_struct 
+      )
+  )
+
+val is_valid_protocol_version: packet_data: (B.buffer U8.t) 
+  -> next_start_index:U32.t
+  -> Stack (protocoll_version_struct: struct_protocol_version)
+    (requires fun h0 -> B.live h0 packet_data)
+    (ensures fun h0 r h1 -> true)
+let is_valid_protocol_version packet_data next_start_index = 
+  (
+    if (not (U8.eq packet_data.(next_start_index) 0x05uy)) then
+      (
+        let protocol_version_struct: struct_protocol_version = {
+          is_valid_protocol_version = false;
+          connect_flag_start_index = 0ul;
+        } in protocol_version_struct
+      )
+    else 
+      (
+        let protocol_version_struct: struct_protocol_version = {
+          is_valid_protocol_version = true;
+          connect_flag_start_index = U32.(next_start_index +^ 1ul);
+        } in protocol_version_struct 
+      )
+  )
+
+val get_connect_flag: packet_data: (B.buffer U8.t) 
+  -> next_start_index:U32.t
+  -> Stack (connect_flag_struct: struct_connect_flag)
+    (requires fun h0 -> B.live h0 packet_data)
+    (ensures fun h0 r h1 -> true)
+let get_connect_flag packet_data next_start_index = 
+  let connect_flag: U8.t = packet_data.(next_start_index) in
+  let connect_flag_struct: struct_connect_flag = {
+    connect_flag_value = connect_flag;
+    keep_alive_start_index = U32.(next_start_index +^ 1ul);
+  } in connect_flag_struct
 
 val connect_packet_parser: packet_data: (B.buffer U8.t) 
   -> packet_size: type_packet_size 
@@ -104,107 +152,40 @@ let connect_packet_parser packet_data packet_size next_start_index =
   let ptr_keep_alive: B.buffer U8.t = B.alloca 0uy 2ul in
   let ptr_connect_topic_length: B.buffer U32.t = B.alloca 0ul 1ul in
   let ptr_connect_property_id: B.buffer U8.t = B.alloca 0uy 1ul in
-  let inv h (i: nat) =
-    B.live h packet_data /\
-    B.live h ptr_is_break /\
-    B.live h ptr_protocol_name_error_status /\
-    B.live h ptr_protocol_version_error_status /\
-    B.live h ptr_connect_flag /\
-    B.live h ptr_keep_alive /\
-    B.live h ptr_connect_topic_length /\
-    B.live h ptr_connect_property_id
-    in
-  let body (i: U32.t{ 2 <= U32.v i && U32.v i < U32.v packet_size  }): Stack unit
-    (requires (fun h -> inv h (U32.v i)))
-    (ensures (fun _ _ _ -> true))
-  =
-    let one_byte : U8.t = packet_data.(i) in
-    let is_break: bool = ptr_is_break.(0ul) in
-    if (is_break) then
-      ()
-    else
-      (
-        let variable_header_index = U32.sub i next_start_index in
-        if (U32.lte variable_header_index 5ul) then
-          (
-            if (
-              (U32.eq variable_header_index 0ul && not (U8.eq one_byte 0x00uy)) ||
-              (U32.eq variable_header_index 1ul && not (U8.eq one_byte 0x04uy)) ||
-              (U32.eq variable_header_index 2ul && not (U8.eq one_byte 0x4Duy)) ||
-              (U32.eq variable_header_index 3ul && not (U8.eq one_byte 0x51uy)) ||
-              (U32.eq variable_header_index 4ul && not (U8.eq one_byte 0x54uy)) ||
-              (U32.eq variable_header_index 5ul && not (U8.eq one_byte 0x54uy))
-              ) then
-              (
-                ptr_protocol_name_error_status.(0ul) <- 1uy;
-                ptr_is_break.(0ul) <- true
-              )
-          )
-          else if (U32.eq variable_header_index 6ul && not (U8.eq one_byte 0x05uy)) then
-            (
-              ptr_protocol_version_error_status.(0ul) <- 1uy;
-              ptr_is_break.(0ul) <- true
-            )
-          else if (U32.eq variable_header_index 7ul) then
-            (
-              ptr_connect_flag.(0ul) <- one_byte
-            )
-          else if (U32.eq variable_header_index 8ul) then
-            (
-              ptr_keep_alive.(0ul) <- one_byte
-            )
-          else if (U32.eq variable_header_index 9ul) then
-            (
-              if (U8.lte one_byte 0x7Fuy) then
-                (
-                  ptr_keep_alive.(1ul) <- one_byte
-                )
-              // else 
-              //   (
-              //     // TODO: keep aliveが127以上の場合は未実装.
-              //   )
-            )
-          else if (U32.eq variable_header_index 10ul) then
-            (
-              // TODO: topic length が一桁かつ, keep aliveが127以下の場合
-              let variable_length: struct_variable_length = 
-                        get_variable_byte packet_data packet_size i in
-              ptr_connect_topic_length.(0ul) <- uint8_to_uint32 one_byte
-            )
-          else if (U32.eq variable_header_index 11ul) then
-            (
-              // TODO: topic length が一桁かつ, keep aliveが127以下の場合
-              ptr_connect_property_id.(0ul) <- one_byte
-            )
-          // else
-          //   (
-          //     print_string "x: ";
-          //     print_u8 one_byte;
-          //     print_string ", index: ";
-          //     print_u32 variable_header_index;
-          //     print_string "\n"
-          //   )
-      )
-  in
-  C.Loops.for next_start_index packet_size inv body;
-
-  let protocol_name_error_status: U8.t = ptr_protocol_name_error_status.(0ul) in
-  let protocol_version_error_status: U8.t = ptr_protocol_version_error_status.(0ul) in
-  let connect_flag: U8.t = ptr_connect_flag.(0ul) in
-  let keep_alive_msb_u8: U8.t = ptr_keep_alive.(0ul) in
-  let keep_alive_lsb_u8: U8.t = ptr_keep_alive.(1ul) in
-  let connect_topic_length: U32.t = ptr_connect_topic_length.(0ul) in
-  let connect_property_id: U8.t = ptr_connect_property_id.(0ul) in
+  let protocol_name_struct: struct_protocol_name = 
+    is_valid_protocol_name packet_data next_start_index in
+  let protocol_version_struct: struct_protocol_version =
+    is_valid_protocol_version packet_data protocol_name_struct.protocol_version_start_index in
+  let connect_flag_struct: struct_connect_flag = 
+    get_connect_flag packet_data protocol_version_struct.connect_flag_start_index in
+  let keep_alive: U16.t = 
+    get_two_byte_integer_u8_to_u16
+      packet_data.(connect_flag_struct.keep_alive_start_index)
+      packet_data.(U32.(connect_flag_struct.keep_alive_start_index +^ 1ul)) in
+  let variable_integer_start_index: U32.t =
+    U32.(connect_flag_struct.keep_alive_start_index +^ 2ul) in
+  let variable_length: struct_variable_length = 
+    get_variable_byte 
+      packet_data packet_size variable_integer_start_index in
+  let property_length: type_remaining_length = 
+    variable_length.variable_length_value in
+  let property_start_index: U32.t = variable_length.next_start_index in
+  let property_struct: struct_property = 
+    parse_property packet_data packet_size property_length property_start_index in
+  let property_type_id = property_struct.property_type_id in
+  let payload_start_index: U32.t = property_struct.payload_start_index in
+  let connect_id: struct_utf8_string = 
+    get_utf8_encoded_string packet_data payload_start_index in
   pop_frame ();
 
   let connect_packet_seed: struct_connect_packet_seed = {
-    connect_seed_protocol_name_error_status = protocol_name_error_status;
-    connect_seed_protocol_version_error_status = protocol_version_error_status;
-    connect_seed_connect_flag = connect_flag;
-    connect_seed_keep_alive_msb_u8 = keep_alive_msb_u8;
-    connect_seed_keep_alive_lsb_u8 = keep_alive_lsb_u8;
-    connect_seed_connect_topic_length = connect_topic_length;
-    connect_seed_connect_property_id = connect_property_id;
+    connect_seed_is_valid_protocol_name = protocol_name_struct.is_valid_protocol_name;
+    connect_seed_is_valid_protocol_version = protocol_version_struct.is_valid_protocol_version;
+    connect_seed_connect_flag = connect_flag_struct.connect_flag_value;
+    connect_seed_keep_alive = keep_alive;
+    connect_seed_is_valid_property_length = not variable_length.have_error;
+    connect_seed_property = property_struct;
+    connect_seed_connect_id = connect_id;
   } in connect_packet_seed
 
 val connect_packet_parse_result: (share_common_data: struct_share_common_data)
@@ -224,36 +205,55 @@ let connect_packet_parse_result share_common_data =
   let will_flag: U8.t = slice_byte connect_flag 5uy 6uy in
   let clean_start_flag: U8.t = slice_byte connect_flag 6uy 7uy in
   let resreved_flag: U8.t = slice_byte connect_flag 7uy 8uy in
-  let connect_property_id: U8.t = connect_packet_seed.connect_seed_connect_property_id in
-  let keep_alive_msb_u32: U32.t = 
-    uint8_to_uint32 connect_packet_seed.connect_seed_keep_alive_msb_u8  in
-  let keep_alive_lsb_u32: U32.t = 
-    uint8_to_uint32 connect_packet_seed.connect_seed_keep_alive_lsb_u8 in 
-  let keep_alive: U32.t = 
-    U32.logor (U32.shift_left keep_alive_msb_u32 8ul)keep_alive_lsb_u32 in
+
+  // let connect_property_id: U8.t = connect_packet_seed.connect_seed_connect_property_id in
+  // let keep_alive_msb_u32: U32.t = 
+  //   uint8_to_uint32 connect_packet_seed.connect_seed_keep_alive_msb_u8  in
+  // let keep_alive_lsb_u32: U32.t = 
+  //   uint8_to_uint32 connect_packet_seed.connect_seed_keep_alive_lsb_u8 in 
+  let keep_alive: U16.t = connect_packet_seed.connect_seed_keep_alive in
 
   let have_error: bool =
-    (connect_packet_seed.connect_seed_protocol_name_error_status = 1uy) ||
-    (connect_packet_seed.connect_seed_protocol_version_error_status = 1uy) ||
-    (not (U8.eq resreved_flag 0uy) ) in
+    (not connect_packet_seed.connect_seed_is_valid_protocol_name) ||
+    (not connect_packet_seed.connect_seed_is_valid_protocol_version) ||
+    (not (U8.eq resreved_flag 0uy)) ||
+    (not connect_packet_seed.connect_seed_is_valid_property_length) ||
+    (U8.gt connect_packet_seed.connect_seed_property.property_type_struct.property_type_error.property_error_code 0uy) ||
+    (U8.gt connect_packet_seed.connect_seed_connect_id.utf8_string_status_code 0uy)
+     in
   if (have_error) then
     (
       let error_struct: struct_error_struct =
         (
-          if (connect_packet_seed.connect_seed_protocol_name_error_status = 1uy) then
+          if (not connect_packet_seed.connect_seed_is_valid_protocol_name) then
             {
               code = define_error_protocol_name_invalid_code;
               message = define_error_protocol_name_invalid;
             }
-          else if (connect_packet_seed.connect_seed_protocol_version_error_status = 1uy) then
+          else if (not connect_packet_seed.connect_seed_is_valid_protocol_version) then
             {
               code = define_error_protocol_version_invalid_code;
               message = define_error_protocol_version_invalid;
             }
-          else // if (not (U8.eq resreved_flag 0uy) ) then
+          else if (not (U8.eq resreved_flag 0uy)) then
             {
               code = define_error_connect_flag_invalid_code;
               message = define_error_connect_flag_invalid;
+            }
+          else if (not connect_packet_seed.connect_seed_is_valid_property_length) then
+            {
+              code = define_error_property_length_invalid_code;
+              message = define_error_property_length_invalid;
+            }
+          else if (U8.gt connect_packet_seed.connect_seed_property.property_type_struct.property_type_error.property_error_code 0uy) then
+            {
+              code = define_error_connect_id_invalid_code;
+              message = connect_packet_seed.connect_seed_property.property_type_struct.property_type_error.property_error_code_name;
+            }
+          else // if (U8.gt connect_packet_seed.connect_id.utf8_string_status_code 0uy)
+            {
+              code = define_error_connect_id_invalid_code;
+              message = define_error_connect_id_invalid;
             }
         ) in error_struct_fixed_header error_struct
     )
@@ -265,8 +265,8 @@ let connect_packet_parse_result share_common_data =
           connect_connect_constant = connect_constant;
           connect_connect_flag = connect_flag;
           connect_keep_alive = keep_alive;
-          connect_connect_topic_length = connect_packet_seed.connect_seed_connect_topic_length;
-          connect_connect_property_id = connect_packet_seed.connect_seed_connect_property_id;
+          connect_property = connect_packet_seed.connect_seed_property;
+          connect_id = connect_packet_seed.connect_seed_connect_id;
       } in
       assemble_connect_struct ed_fixed_header_parts            
     )
